src/opt/AdequacyThread.v
@@ -15,7 +15,307 @@ Require Import Configuration.
 
 Require Import SimMemory.
 Require Import SimPromises.
+Require Import SimLocal.
 Require Import SimThread.
 Require Import Simulation.
 
 Set Implicit Arguments.
+
+
+Lemma tids_find
+      tids ths_src ths_tgt
+      tid
+      (TIDS_SRC: tids = Threads.tids ths_src)
+      (TIDS_TGT: tids = Threads.tids ths_tgt):
+  (exists lang_src st_src lc_src, IdentMap.find tid ths_src = Some (existT _ lang_src st_src, lc_src)) <->
+  (exists lang_tgt st_tgt lc_tgt, IdentMap.find tid ths_tgt = Some (existT _ lang_tgt st_tgt, lc_tgt)).
+Proof.
+  split; i; des.
+  - destruct (IdentSet.mem tid tids) eqn:MEM.
+    + rewrite TIDS_TGT in MEM.
+      rewrite Threads.tids_o in MEM.
+      destruct (IdentMap.find tid ths_tgt); ss.
+      destruct p. destruct s. esplits; eauto.
+    + rewrite TIDS_SRC in MEM.
+      rewrite Threads.tids_o in MEM.
+      destruct (IdentMap.find tid ths_src); ss.
+  - destruct (IdentSet.mem tid tids) eqn:MEM.
+    + rewrite TIDS_SRC in MEM.
+      rewrite Threads.tids_o in MEM.
+      destruct (IdentMap.find tid ths_src); ss.
+      destruct p. destruct s. esplits; eauto.
+    + rewrite TIDS_TGT in MEM.
+      rewrite Threads.tids_o in MEM.
+      destruct (IdentMap.find tid ths_tgt); ss.
+Qed.
+
+Lemma thread_rtc_step_rtc_step
+      l
+      ths1_src sc1_src mem1_src
+      sc2_src mem2_src
+      ths_tgt sc_tgt mem_tgt
+      tid lang_src st1_src lc1_src st2_src lc2_src
+      (TIDS: Threads.tids ths1_src = Threads.tids ths_tgt)
+      (NOTIN: forall tid' lang_src st_src lc_src
+                (FIND: IdentMap.find tid' ths1_src = Some (existT _ lang_src st_src, lc_src))
+                (TID: ~ (tid = tid' \/ List.In tid' l)),
+          Language.is_terminal _ st_src /\ Local.is_terminal lc_src)
+      (IN: forall tid' lang_src st_src lc_src lang_tgt st_tgt lc_tgt
+             (TID: tid = tid' \/ List.In tid' l),
+          IdentMap.find tid' ths1_src = Some (existT _ lang_src st_src, lc_src) ->
+          IdentMap.find tid' ths_tgt = Some (existT _ lang_tgt st_tgt, lc_tgt) ->
+          exists sim_terminal,
+            @sim_thread lang_src lang_tgt sim_terminal st_src lc_src sc1_src mem1_src st_tgt lc_tgt sc_tgt mem_tgt)
+      (WF_SRC: Configuration.wf (Configuration.mk ths1_src sc1_src mem1_src))
+      (WF_TGT: Configuration.wf (Configuration.mk ths_tgt sc_tgt mem_tgt))
+      (CONSISTENT_TGT: Configuration.consistent (Configuration.mk ths_tgt sc_tgt mem_tgt))
+      (FIND: IdentMap.find tid ths1_src = Some (existT _ lang_src st1_src, lc1_src))
+      (STEPS: rtc (@Thread.tau_step lang_src)
+                  (Thread.mk lang_src st1_src lc1_src sc1_src mem1_src)
+                  (Thread.mk lang_src st2_src lc2_src sc2_src mem2_src))
+      (MEMORY2: sim_memory mem2_src mem_tgt)
+      (SC2: TimeMap.le sc2_src sc_tgt)
+      (LOCAL: Local.promises lc2_src = Memory.bot):
+  rtc Configuration.tau_step
+      (Configuration.mk ths1_src sc1_src mem1_src)
+      (Configuration.mk (IdentMap.add tid (existT _ lang_src st2_src, lc2_src) ths1_src) sc2_src mem2_src).
+Proof.
+  inv WF_SRC. inv WF. ss. exploit THREADS; eauto. i.
+  exploit Thread.rtc_tau_step_future; eauto. s. i. des.
+  generalize (rtc_tail STEPS). i. des.
+  - inv H0. inv TSTEP. econs; eauto.
+    econs. rewrite <- EVENT. econs; ss; eauto.
+    unfold Configuration.consistent. s.
+    unfold Threads.consistent. i.
+    destruct (Ident.eq_dec tid0 tid).
+    + subst. rewrite IdentMap.gss in TH.
+      inv TH. Configuration.simplify.
+      ii. ss. esplits; eauto.
+    + rewrite IdentMap.gso in TH; auto.
+      destruct (List.In_dec Ident.eq_dec tid0 l); cycle 1.
+      { exploit NOTIN; eauto.
+        { ii. des; ss. subst. ss. }
+        i. des. ii. esplits; eauto. ss. apply x1. }
+      destruct (IdentMap.find tid0 ths_tgt) as [[[lang_tgt st_tgt] lc_tgt]|] eqn:FIND_TGT; cycle 1.
+      { remember (Threads.tids ths1_src) as tids eqn:TIDS_SRC.
+        exploit tids_find; [exact TIDS_SRC|exact TIDS|..]. i. des.
+        exploit x1; eauto. i. des. rewrite FIND_TGT in x3. inv x3. }
+      exploit IN; eauto. i. des.
+      exploit sim_thread_future; try exact x0; try exact SC_FUTURE; try exact MEM_FUTURE; try refl; eauto. i.
+      inv WF_TGT. inv WF. ss. exploit THREADS0; eauto. i.
+      hexploit sim_thread_consistent; try exact x2; eauto.
+      exploit Thread.rtc_tau_step_disjoint; eauto. s. i. des.
+      exploit Thread.rtc_tau_step_future; eauto. s. i. des.
+      exploit Thread.step_disjoint; eauto. s. i. des.
+      auto.
+  - inv H.
+    replace (IdentMap.add tid (existT _ lang_src st2_src, lc2_src) ths1_src) with ths1_src; auto.
+    apply IdentMap.eq_leibniz. ii.
+    rewrite -> IdentMap.gsident; auto.
+Qed.
+
+Lemma sim_thread_sim
+      ths_src sc0_src mem0_src
+      ths_tgt sc0_tgt mem0_tgt
+      (TIDS: Threads.tids ths_src = Threads.tids ths_tgt)
+      (SIM: forall tid lang_src st_src lc_src lang_tgt st_tgt lc_tgt,
+          IdentMap.find tid ths_src = Some (existT _ lang_src st_src, lc_src) ->
+          IdentMap.find tid ths_tgt = Some (existT _ lang_tgt st_tgt, lc_tgt) ->
+          exists sim_terminal,
+            @sim_thread lang_src lang_tgt sim_terminal st_src lc_src sc0_src mem0_src st_tgt lc_tgt sc0_tgt mem0_tgt)
+  :
+    sim ths_src sc0_src mem0_src ths_tgt sc0_tgt mem0_tgt.
+Proof.
+  remember (Threads.tids ths_src) as tids eqn:TIDS_SRC.
+  rename TIDS into TIDS_TGT.
+  revert ths_src sc0_src mem0_src ths_tgt sc0_tgt mem0_tgt tids TIDS_SRC TIDS_TGT SIM.
+  pcofix CIH. i. pfold. ii. splits.
+  - (* TERMINAL CASE *)
+    assert (NOTIN: forall tid lang_src st_src lc_src
+                     (FIND: IdentMap.find tid ths_src = Some (existT _ lang_src st_src, lc_src))
+                     (TID: ~ List.In tid (IdentSet.elements tids)),
+               Language.is_terminal _ st_src /\ Local.is_terminal lc_src).
+    { i. destruct (IdentSet.mem tid tids) eqn:MEM.
+      - exfalso. apply TID. rewrite IdentSet.mem_spec in MEM.
+        rewrite <- IdentSet.elements_spec1 in MEM.
+        clear - MEM. induction MEM; [econs 1|econs 2]; auto.
+      - rewrite TIDS_SRC in MEM. rewrite Threads.tids_o in MEM.
+        destruct (IdentMap.find tid ths_src) eqn:IFIND; [inv MEM|]. ss. }
+    assert (IN: forall tid lang_src st_src lc_src lang_tgt st_tgt lc_tgt
+                  (TID: List.In tid (IdentSet.elements tids)),
+               IdentMap.find tid ths_src = Some (existT _ lang_src st_src, lc_src) ->
+               IdentMap.find tid ths_tgt = Some (existT _ lang_tgt st_tgt, lc_tgt) ->
+               exists sim_terminal,
+                 @sim_thread lang_src lang_tgt sim_terminal st_src lc_src sc0_src mem0_src st_tgt lc_tgt sc0_tgt mem0_tgt).
+    { eauto. }
+    assert (TIDS_MEM: forall tid, List.In tid (IdentSet.elements tids) -> IdentSet.mem tid tids = true).
+    { i. rewrite IdentSet.mem_spec.
+      rewrite <- IdentSet.elements_spec1.
+      eapply SetoidList.In_InA; auto. }
+    assert (NODUP: List.NoDup (IdentSet.elements tids)).
+    { specialize (IdentSet.elements_spec2w tids). i.
+      clear - H. induction H; econs; eauto. }
+    revert NOTIN IN TIDS_MEM NODUP.
+    move tids at top. clear SIM. revert_until CIH.
+    induction (IdentSet.elements tids); i.
+    { esplits; eauto. ii. exploit NOTIN; eauto. }
+    destruct (IdentMap.find a ths_src) as [[[lang_src st_src] lc_src]|] eqn:ASRC;
+      destruct (IdentMap.find a ths_tgt) as [[[lang_tgt st_tgt] lc_tgt]|] eqn:ATGT; cycle 1.
+    { exploit tids_find; [apply TIDS_SRC|apply TIDS_TGT|..]. i. des.
+      exploit x0; eauto. i. des. rewrite ATGT in x. inv x. }
+    { exploit tids_find; [apply TIDS_SRC|apply TIDS_TGT|..]. i. des.
+      exploit x1; eauto. i. des. rewrite ASRC in x. inv x. }
+    { exploit IHl; [exact TIDS_SRC|exact TIDS_TGT|exact SC1|exact MEMORY1|..]; eauto; i.
+      - eapply NOTIN; eauto. ii. inv H; ss. congr.
+      - eapply IN; eauto. econs 2; eauto.
+      - eapply TIDS_MEM; eauto. econs 2; eauto.
+      - inv NODUP. ss.
+    }
+    generalize WF_SRC. intro X. inv X. ss. inv WF. exploit THREADS; eauto. i.
+    generalize WF_TGT. intro X. inv X. ss. inv WF. exploit THREADS0; eauto. i.
+    exploit (IN a); eauto. i. des.
+    exploit TERMINAL_TGT; eauto. i. des.
+    punfold x2. exploit x2; try exact x; try exact x0; try exact SC; try exact SC0; eauto. i. des.
+    exploit TERMINAL; eauto. i. des.
+    exploit thread_rtc_step_rtc_step; try exact STEPS; eauto; i.
+    { guardH TID. exploit IN; try eapply TID; eauto. i. des.
+      esplits. eapply sim_thread_future; try exact x1; eauto. }
+    { inv THREAD. eapply sim_local_memory_bot; eauto. }
+    exploit Configuration.rtc_step_future; try eapply x3; eauto. s. i. des.
+    exploit IHl; [| |exact SC2|exact MEMORY|..]; try exact WF2; try exact WF_TGT;
+      try exact SC_FUTURE_TGT; try exact MEM_FUTURE_TGT;
+        try (etrans; [exact SC_FUTURE_SRC|exact SC_FUTURE]);
+        try (etrans; [exact MEM_FUTURE_SRC|exact MEM_FUTURE]); eauto; i.
+    { rewrite Threads.tids_add. rewrite IdentSet.add_mem; eauto. }
+    { rewrite IdentMap.gsspec in FIND. revert FIND. condtac; ss; i.
+      - subst. Configuration.simplify. split; auto.
+        inv THREAD. econs. eapply sim_local_memory_bot; eauto.
+      - eapply NOTIN; eauto. ii. des; ss. subst. ss. }
+    { rewrite IdentMap.gsspec in H. revert H. condtac; ss; i.
+      - subst. inv NODUP. congr.
+      - exploit IN; eauto. }
+    { inv NODUP. ss. }
+    des. rewrite x1 in x3.
+    esplits; try exact x3; eauto.
+  - (* STEP CASE *)
+    i. inv STEP_TGT. destruct e2. ss.
+    destruct (IdentMap.find tid_tgt ths_src) as [[[lang_src st_src] lc_src]|] eqn:FIND_SRC; cycle 1.
+    { remember (Threads.tids ths_src) as tids eqn:TIDS_SRC.
+      exploit tids_find; [exact TIDS_SRC|exact TIDS_TGT|..]. i. des.
+      exploit x1; eauto. i. des. rewrite FIND_SRC in x. inv x. }
+    inv WF_SRC. inv WF_TGT. inv WF. inv WF0. ss.
+    exploit SIM; eauto. i. des.
+    exploit sim_thread_future; eauto. i.
+    exploit sim_thread_plus_step; try exact STEPS; try exact x1; eauto. s. i. des.
+    inv STEP0.
+    + generalize (rtc_tail STEPS0). intro X. des.
+      * inv X0. inv TSTEP. esplits; eauto.
+        { rewrite <- EVENT. ss. rewrite <- EVENT0.
+          econs 2. econs; eauto. ss.
+          unfold Configuration.consistent. s.
+          unfold Threads.consistent. i.
+          rewrite IdentMap.gsspec in TH. revert TH. condtac; ss; i.
+          - inv TH. Configuration.simplify.
+            eapply sim_thread_consistent; eauto.
+            eapply CONSISTENT; ss. rewrite IdentMap.gss. ss.
+          - destruct (IdentMap.find tid ths_tgt) as [[[lang_tgt st_tgt] lc_tgt]|] eqn:FIND_TGT; cycle 1.
+            { remember (Threads.tids ths_src) as tids eqn:TIDS_SRC.
+              exploit tids_find; [exact TIDS_SRC|exact TIDS_TGT|..]. i. des.
+              exploit x2.
+              { esplits; eapply TH. }
+              i. des. rewrite FIND_TGT in x4. inv x4. }
+            exploit SIM; eauto. i. des.
+            exploit sim_thread_future; try exact x0; eauto. i.
+            exploit Thread.rtc_tau_step_future; try exact STEPS; eauto. s. i. des.
+            exploit Thread.step_future; try exact STEP; eauto. s. i. des.
+            exploit Thread.rtc_tau_step_future; try exact STEPS0; eauto. s. i. des.
+            exploit sim_thread_future; try exact x3;
+              try exact SC_FUTURE1; try exact MEM_FUTURE1; try (etrans; eauto). i.
+            eapply sim_thread_consistent; try exact x4; eauto.
+            { exploit THREADS; eauto. i.
+              exploit DISJOINT; [|exact FIND_SRC|exact TH|]; eauto. i.
+              exploit Thread.rtc_tau_step_disjoint; try exact STEPS0; eauto. s. i. des. ss. }
+            { exploit THREADS0; eauto. i.
+              exploit DISJOINT0; [|exact TID|exact FIND_TGT|]; eauto. i.
+              exploit Thread.rtc_tau_step_disjoint; try exact STEPS; eauto. s. i. des.
+              exploit Thread.step_disjoint; try exact STEP; eauto. s. i. des. ss. }
+            { eapply CONSISTENT. s. rewrite IdentMap.gso; eauto. }
+        }
+        { ss. right. eapply CIH.
+          - rewrite Threads.tids_add. rewrite IdentSet.add_mem; ss.
+            rewrite Threads.tids_o. rewrite FIND_SRC. ss.
+          - rewrite TIDS_TGT.
+            rewrite Threads.tids_add. rewrite IdentSet.add_mem; ss.
+            rewrite Threads.tids_o. rewrite TID. ss.
+          - i. Configuration.simplify; [eexists; eauto|].
+            exploit Thread.rtc_tau_step_future; try exact STEPS; eauto. s. i. des.
+            exploit Thread.step_future; try exact STEP; eauto. s. i. des.
+            exploit Thread.rtc_tau_step_future; try exact X; eauto. s. i. des.
+            exploit Thread.step_future; try exact STEP0; eauto. s. i. des.
+            exploit SIM; try eapply H; eauto. i. des.
+            eexists.
+            eapply sim_thread_future; try exact x0; try by (etrans; [eauto|etrans; eauto]). }
+      * ss. inv X. esplits; eauto.
+        { destruct e0; ss. }
+        { right. eapply CIH; ss.
+          - rewrite TIDS_TGT.
+            rewrite Threads.tids_add. rewrite IdentSet.add_mem; ss.
+            rewrite Threads.tids_o. rewrite TID. ss.
+          - i. Configuration.simplify.
+            + rewrite FIND_SRC in H. inv H. Configuration.simplify.
+              eexists; eauto.
+            + exploit Thread.rtc_tau_step_future; try exact STEPS; eauto. s. i. des.
+              exploit Thread.step_future; try exact STEP; eauto. s. i. des.
+              exploit SIM; try eapply H; eauto. i. des.
+              eexists.
+              eapply sim_thread_future; try exact x0; eauto; try by (etrans; [eauto|etrans; eauto]). }
+    + esplits; eauto.
+      * rewrite <- EVENT.
+        econs 2. econs; eauto. ss.
+        unfold Configuration.consistent. s.
+        unfold Threads.consistent. i.
+        rewrite IdentMap.gsspec in TH. revert TH. condtac; ss; i.
+        { inv TH. Configuration.simplify.
+          eapply sim_thread_consistent; eauto.
+          eapply CONSISTENT; ss. rewrite IdentMap.gss. ss. }
+        { destruct (IdentMap.find tid ths_tgt) as [[[lang_tgt st_tgt] lc_tgt]|] eqn:FIND_TGT; cycle 1.
+          { remember (Threads.tids ths_src) as tids eqn:TIDS_SRC.
+            exploit tids_find; [exact TIDS_SRC|exact TIDS_TGT|..]. i. des.
+            exploit x2.
+            { esplits; eapply TH. }
+            i. des. rewrite FIND_TGT in x4. inv x4. }
+          exploit SIM; eauto. i. des.
+          exploit sim_thread_future; try exact x0; eauto. i.
+          exploit Thread.rtc_tau_step_future; try exact STEPS; eauto. s. i. des.
+          exploit Thread.step_future; try exact STEP; eauto. s. i. des.
+          exploit Thread.rtc_tau_step_future; try exact STEPS0; eauto. s. i. des.
+          exploit Thread.step_future; try exact STEP1; eauto. s. i. des.
+          exploit sim_thread_future; try exact x3; try by etrans; eauto. i.
+          eapply sim_thread_consistent; try exact x4; eauto.
+          { exploit THREADS; eauto. i.
+            exploit DISJOINT; [|exact FIND_SRC|exact TH|]; eauto. i.
+            exploit Thread.rtc_tau_step_disjoint; try exact STEPS0; eauto. s. i. des.
+            exploit Thread.step_disjoint; try exact STEP1; eauto. s. i. des. ss. }
+          { exploit THREADS0; eauto. i.
+            exploit DISJOINT0; [|exact TID|exact FIND_TGT|]; eauto. i.
+            exploit Thread.rtc_tau_step_disjoint; try exact STEPS; eauto. s. i. des.
+            exploit Thread.step_disjoint; try exact STEP; eauto. s. i. des. ss. }
+          { eapply CONSISTENT. s. rewrite IdentMap.gso; eauto. }
+        }
+      * ss. right. eapply CIH.
+        { rewrite Threads.tids_add. rewrite IdentSet.add_mem; ss.
+          rewrite Threads.tids_o. rewrite FIND_SRC. ss. }
+        { rewrite TIDS_TGT.
+          rewrite Threads.tids_add. rewrite IdentSet.add_mem; ss.
+          rewrite Threads.tids_o. rewrite TID. ss. }
+        { i. Configuration.simplify; [eexists; eauto|].
+          exploit Thread.rtc_tau_step_future; try exact STEPS; eauto. s. i. des.
+          exploit Thread.step_future; try exact STEP; eauto. s. i. des.
+          exploit Thread.rtc_tau_step_future; try exact STEPS0; eauto. s. i. des.
+          exploit Thread.step_future; try exact STEP1; eauto. s. i. des.
+          exploit SIM; try eapply H; eauto. i. des.
+          eexists.
+          eapply sim_thread_future; try exact x0; try by (etrans; [eauto|etrans; eauto]). }
+Grab Existential Variables.
+  { auto. }
+Qed.
